Remove string cruft that's been upstreamed
Since we now no longer support Coq 8.8, we can rely on definitions in
the standard library to print and parse strings.

The upshot is that now we have many fewer lines of code, and we have a
couple more proofs about the fact that `parse ∘ print` is the identity.

src/Util/Strings/String.v
@@ -1,48 +1,46 @@
 Require Import Coq.omega.Omega.
 Require Import Coq.Strings.String.
 Require Import Coq.Strings.Ascii.
-Require Import Crypto.Util.Strings.Equality.
 Require Import Crypto.Util.Strings.Ascii.
 
 Local Open Scope list_scope.
 Local Open Scope string_scope.
 
-(** *** String concatenation *)
-(** [concat sep sl] concatenates the list of strings [sl], inserting
-    the separator string [sep] between each. *)
 
-Definition concat (sep : string) : list string -> string
-  := fix concat (sl : list string) : string
-       := match sl with
-          | nil => EmptyString
-          | cons x nil => x
-          | cons x xs => x ++ sep ++ concat xs
-          end.
+(** TODO: Remove this once we drop support for Coq 8.9 (it's in the stdlib in Coq 8.10 *)
+(** *** Conversion to/from [list ascii] *)
 
-(** *** Conversion to and from lists *)
-Fixpoint to_list (s : string) : list ascii
-  := match s with
-     | EmptyString => nil
-     | String x xs => cons x (to_list xs)
-     end.
-Fixpoint of_list (s : list ascii) : string
+Fixpoint string_of_list_ascii (s : list ascii) : string
   := match s with
      | nil => EmptyString
-     | cons x xs => String x (of_list xs)
+     | cons ch s => String ch (string_of_list_ascii s)
      end.
 
-Lemma to_of_list s : to_list (of_list s) = s.
-Proof. induction s as [|x xs IHxs]; cbn; [ | rewrite IHxs ]; reflexivity. Qed.
-Lemma of_to_list s : of_list (to_list s) = s.
-Proof. induction s as [|x xs IHxs]; cbn; [ | rewrite IHxs ]; reflexivity. Qed.
+Fixpoint list_ascii_of_string (s : string) : list ascii
+  := match s with
+     | EmptyString => nil
+     | String ch s => cons ch (list_ascii_of_string s)
+     end.
 
-Lemma of_list_app s1 s2 : of_list (s1 ++ s2) = of_list s1 ++ of_list s2.
+Lemma string_of_list_ascii_of_string s : string_of_list_ascii (list_ascii_of_string s) = s.
+Proof.
+  induction s as [|? ? IHs]; [ reflexivity | cbn; apply f_equal, IHs ].
+Defined.
+
+Lemma list_ascii_of_string_of_list_ascii s : list_ascii_of_string (string_of_list_ascii s) = s.
+Proof.
+  induction s as [|? ? IHs]; [ reflexivity | cbn; apply f_equal, IHs ].
+Defined.
+
+(** *** String concatenation *)
+
+Lemma string_of_list_ascii_app s1 s2 : string_of_list_ascii (s1 ++ s2) = string_of_list_ascii s1 ++ string_of_list_ascii s2.
 Proof. induction s1 as [|x xs IHxs]; cbn; [ | rewrite IHxs ]; reflexivity. Qed.
-Lemma to_list_app s1 s2 : to_list (s1 ++ s2) = (to_list s1 ++ to_list s2)%list.
+Lemma list_ascii_of_string_app s1 s2 : list_ascii_of_string (s1 ++ s2) = (list_ascii_of_string s1 ++ list_ascii_of_string s2)%list.
 Proof. induction s1 as [|x xs IHxs]; cbn; [ | rewrite IHxs ]; reflexivity. Qed.
 
 Definition lift_list_function (f : list ascii -> list ascii) (s : string) : string
-  := of_list (f (to_list s)).
+  := string_of_list_ascii (f (list_ascii_of_string s)).
 
 (** *** Mapping over a string *)
 (** [map f s] applies function [f] in turn to all the characters of
@@ -72,7 +70,7 @@ Lemma rev_step s
       | EmptyString => EmptyString
       | String x xs => rev xs ++ String x EmptyString
       end.
-Proof. destruct s; cbn; rewrite ?of_list_app; reflexivity. Qed.
+Proof. destruct s; cbn; rewrite ?string_of_list_ascii_app; reflexivity. Qed.
 
 (** *** trimming a string *)
 (** [trim s] returns a copy of the argument, without leading and trailing
@@ -103,15 +101,15 @@ Definition rindex (n : nat) (s1 s2 : string) : option nat :=
     (index (length s2 - n - 1) (rev s1) (rev s2)).
 
 
-Lemma append_alt s1 s2 : s1 ++ s2 = of_list (to_list s1 ++ to_list s2).
-Proof. rewrite of_list_app, !of_to_list; reflexivity. Qed.
+Lemma append_alt s1 s2 : s1 ++ s2 = string_of_list_ascii (list_ascii_of_string s1 ++ list_ascii_of_string s2).
+Proof. rewrite string_of_list_ascii_app, !string_of_list_ascii_of_string; reflexivity. Qed.
 Lemma append_empty_r s : s ++ "" = s.
 Proof.
-  rewrite append_alt; cbn; rewrite List.app_nil_r, of_to_list. reflexivity.
+  rewrite append_alt; cbn; rewrite List.app_nil_r, string_of_list_ascii_of_string. reflexivity.
 Qed.
 Lemma append_assoc s1 s2 s3 : s1 ++ (s2 ++ s3) = (s1 ++ s2) ++ s3.
 Proof.
-  rewrite !append_alt, ?to_of_list; cbn; rewrite List.app_assoc; reflexivity.
+  rewrite !append_alt, !list_ascii_of_string_of_list_ascii; cbn; rewrite List.app_assoc; reflexivity.
 Qed.
 
 Lemma length_substring n1 n2 s
@@ -143,10 +141,9 @@ Definition startswith (prefix s : string) : bool
 Lemma startswith_correct prefix s
   : startswith prefix s = true <-> substring 0 (length prefix) s = prefix.
 Proof.
+  pose proof (String.eqb_spec prefix (substring 0 (length prefix) s)) as H'.
   cbv [startswith].
-  split; intro H.
-  { apply internal_string_dec_bl in H; congruence. }
-  { apply internal_string_dec_lb; congruence. }
+  split; intro H; destruct H'; congruence.
 Qed.
 
 (** [endswith postfix s] returns [true] iff [s] ends with [postfix] *)
@@ -156,10 +153,9 @@ Definition endswith (postfix s : string) : bool
 Lemma endswith_correct postfix s
   : endswith postfix s = true <-> substring (length s - length postfix) (length postfix) s = postfix.
 Proof.
+  pose proof (String.eqb_spec postfix (substring (length s - length postfix) (length postfix) s)) as H'.
   cbv [endswith].
-  split; intro H.
-  { apply internal_string_dec_bl in H; congruence. }
-  { apply internal_string_dec_lb; congruence. }
+  split; intro H; destruct H'; congruence.
 Qed.
 
 Section strip_prefix_cps.
@@ -170,7 +166,7 @@ Section strip_prefix_cps.
     := match s2 with
        | EmptyString => remaining (String sepch sep) s2
        | String x xs
-         => if ascii_beq sepch x
+         => if (sepch =? x)%char
             then match sep with
                  | EmptyString => found xs
                  | String sepch sep
@@ -195,7 +191,7 @@ End strip_prefix_cps.
 
     - No string in the result contains [sep] as a substring, unless
       [sep] is the empty string, in which case this function returns
-      [map (fun ch => String ch "") (to_list s)] if [s] is non-empty,
+      [map (fun ch => String ch "") (list_ascii_of_string s)] if [s] is non-empty,
       and [""::nil] if [s] is also empty. *)
 
 Fixpoint split_helper (sepch : ascii) (sep : string) (s : string) (rev_acc : string) {struct s}
@@ -213,9 +209,9 @@ Fixpoint split_helper (sepch : ascii) (sep : string) (s : string) (rev_acc : str
 Definition split (sep : string) (s : string) : list string
   := match sep with
      | EmptyString
-       => if string_beq s EmptyString
+       => if (s =? "")%string
           then "" :: nil
-          else List.map (fun ch => String ch "") (to_list s)
+          else List.map (fun ch => String ch "") (list_ascii_of_string s)
      | String sepch sep
        => split_helper sepch sep s ""
      end.
@@ -248,7 +244,7 @@ Lemma split_empty_empty : split EmptyString EmptyString = "" :: nil.
 Proof. reflexivity. Qed.
 Lemma split_empty_non_empty s
   : s <> EmptyString
-    -> split EmptyString s = List.map (fun ch => String ch "") (to_list s).
+    -> split EmptyString s = List.map (fun ch => String ch "") (list_ascii_of_string s).
 Proof.
   intro H; destruct s; cbn; congruence.
 Qed.
@@ -295,14 +291,13 @@ Proof.
   fix H' 3.
   intros sepch' sep' s'; intros.
   destruct s' as [|a s']; cbn; [ assumption | ].
-  destruct (sepch' =? a)%char eqn:Hsep, sep'; try (clear H' concat_split_helper; congruence).
+  destruct (Ascii.eqb_spec sepch' a), sep'; try (clear H' concat_split_helper; congruence).
   { cbn [concat].
     rewrite (concat_split_helper sepch' "" s').
     destruct (split_helper sepch' "" s' "") eqn:H''.
     { apply split_helper_non_empty in H''; exfalso; assumption. }
-    { cbn.
-      apply internal_ascii_dec_bl in Hsep; subst; reflexivity. } }
-  { apply internal_ascii_dec_bl in Hsep; subst.
+    { cbn; subst; reflexivity. } }
+  { subst.
 Abort.
 
 Lemma concat_split sep s : concat sep (split sep s) = s.
