src/Util/Strings/Equality.v
@@ -1,9 +1,0 @@
-Require Import Coq.Strings.Ascii Coq.Strings.String.
-Require Import Crypto.Util.Bool.Equality.
-Require Import Crypto.Util.Notations.
-
-Scheme Equality for ascii.
-Scheme Equality for string.
-
-Infix "=?" := ascii_beq : char_scope.
-Infix "=?" := string_beq : string_scope.
